lots of progress on insert_BST except for some lean technicalities

lean/Splay.lean
@@ -1,12 +1,21 @@
 import Mathlib.Tactic.Linarith
 
-def hello := "splay"
+local macro "have_eq " lhs:term:max rhs:term:max : tactic =>
+  `(tactic|
+    (have h : $lhs = $rhs :=
+       -- TODO: replace with linarith
+       by simp_arith at *; apply Nat.le_antisymm <;> assumption
+     try subst $lhs))
+
+local macro "by_cases' " e:term:max h:Lean.binderIdent : tactic =>
+  `(tactic| by_cases $e <;> rename_i $h <;> simp [*])
 
 inductive STree (α : Type u) where
   | leaf
   | node (left : STree α) (key : Nat) (value : α) (right : STree α)
 
 -- TODO doc
+@[simp]
 def STree.splay (tree : STree α) (key : Nat) : STree α :=
   match tree with
   | leaf => leaf
@@ -44,43 +53,48 @@ def STree.splay (tree : STree α) (key : Nat) : STree α :=
             node (node (node l k v rl) rk rv rrl) rrk rrv rrr
 
 -- TODO doc
-def STree.bound (tree : STree α) (key : Nat) : Bool :=
+@[simp]
+def STree.bound' (tree : STree α) (key : Nat) : Bool :=
   match tree with
   | leaf => false
   | node l k _ r =>
     if key = k then true
-    else if key < k then l.bound key
-    else r.bound key
+    else if key < k then l.bound' key
+    else r.bound' key
 
 -- TODO doc
 -- implementing this in terms of splay is possible but it makes it hard to prove
 -- things about it
-def STree.bound' (tree : STree α) (key : Nat) : Bool :=
+@[simp]
+def STree.bound (tree : STree α) (key : Nat) : Bool :=
   match tree.splay key with
   | leaf => false
   | node _ k _ _ => key = k
 
 -- TODO doc
 -- lookup for normal BSTs
-def STree.lookup_aux (tree : STree α) (d : α) (key : Nat) : α :=
+@[simp]
+def STree.lookup_aux (tree : STree α) (key : Nat) : Option α :=
   match tree with
-  | leaf => d
+  | leaf => none
   | node l k v r =>
-    if key = k then v
-    else if key < k then l.lookup_aux d key
-    else r.lookup_aux d key
+    if key = k then some v
+    else if key < k then l.lookup_aux key
+    else r.lookup_aux key
 
 -- TODO doc
 -- easier to prove things this way
-def STree.lookup (tree : STree α) (d : α) (key : Nat) : α × STree α :=
-  (tree.lookup_aux d key, tree.splay key)
+@[simp]
+def STree.lookup' (tree : STree α) (key : Nat) : Option α × STree α :=
+  (tree.lookup_aux key, tree.splay key)
 
-def STree.lookup' (tree : STree α) (d : α) (key : Nat) : α × STree α :=
+@[simp]
+def STree.lookup (tree : STree α) (key : Nat) : Option α × STree α :=
   match tree.splay key with
-  | leaf => (d, leaf)
+  | leaf => (none, leaf)
   | node l k v r =>
-    if key = k then (v, node l k v r) else
-      (d, node l k v r)
+    if key = k then (some v, node l k v r) else
+      (none, node l k v r)
 
 -- TODO doc
 -- insert for normal bst
@@ -152,25 +166,51 @@ theorem splay_zig_zag : splay T5 y = T6 := by rfl
 theorem splay_zag_zig : splay T7 y = T6 := by rfl
 end Tests
 
----- TODO section the bst invariant ----
+---- TODO section the bst invariant, proving insert_BST ----
 
 -- TODO doc
 inductive ForallTree (p : Nat -> α -> Prop) : STree α -> Prop
   | leaf : ForallTree p .leaf
-  | node :
-    ForallTree p left ->
-    p key value ->
-    ForallTree p right ->
-    ForallTree p (.node left key value right)
+  | node : ∀ l k v r,
+    ForallTree p l ->
+    p k v ->
+    ForallTree p r ->
+    ForallTree p (.node l k v r)
 
 -- TODO doc
-inductive BST : STree α -> Prop
+inductive BST {α : Type u} : STree α -> Prop
   | leaf : BST .leaf
-  | node :
-    ForallTree (fun k _ => k < key) left ->
-    ForallTree (fun k _ => k > key) right ->
-    BST left -> BST right ->
-    BST (.node left key value right)
+  | node : ∀ l k v r,
+    ForallTree (fun k' _ => k' < k) l ->
+    ForallTree (fun k' _ => k' > k) r ->
+    BST l -> BST r ->
+    BST (.node l k v r)
+
+inductive splayBST {α : Type u} : STree α -> Prop
+  | leaf : splayBST .leaf
+  | node_e : ∀ k v, splayBST (.node .leaf k v .leaf)
+  | node_l : ∀ k v ll lk lv lr,
+    ForallTree (fun k' _ => k' < lk) ll ->
+    ForallTree (fun k' _ => k' > lk) lr ->
+    ForallTree (fun k' _ => k' < k) (.node ll lk lv lr) ->
+    splayBST ll -> splayBST lr ->
+    splayBST (.node (.node ll lk lv lr) k v .leaf)
+  | node_r : ∀ k v rl rk rv rr,
+    ForallTree (fun k _ => k < rk) rl ->
+    ForallTree (fun k _ => k > rk) rr ->
+    ForallTree (fun k' _ => k' > k) (.node rl rk rv rr) ->
+    splayBST rl -> splayBST rr ->
+    splayBST (.node .leaf k v (.node rl rk rv rr))
+  | node_rl : ∀ k v ll lk lv lr rl rk rv rr,
+    ForallTree (fun k _ => k < lk) ll ->
+    ForallTree (fun k _ => k > lk) lr ->
+    ForallTree (fun k _ => k < rk) rl ->
+    ForallTree (fun k _ => k > rk) rr ->
+    ForallTree (fun k' _ => k' < k) (.node ll lk lv lr) ->
+    ForallTree (fun k' _ => k' > k) (.node rl rk rv rr) ->
+    splayBST ll -> splayBST lr ->
+    splayBST rl -> splayBST rr ->
+    splayBST (.node (.node ll lk lv lr) k v (.node rl rk rv rr))
 
 theorem ForallTree_imp (p q : Nat -> α -> Prop) (t : STree α) :
   ForallTree p t ->
@@ -205,4 +245,475 @@ theorem ForallTree_less (t : STree α) (k k0 : Nat) :
   . assumption
   . intro key _ h3
     linarith
+
+theorem STree.inductionOn
+  {motive : STree α -> Sort u}
+  (base : motive leaf)
+  (ind_te : ∀ k v, motive (node leaf k v leaf))
+  (ind_tl : ∀ k v ll lk lv lr,
+    motive ll -> motive lr ->
+    motive (node (node ll lk lv lr) k v leaf))
+  (ind_tr : ∀ k v rl rk rv rr,
+    motive rl -> motive rr ->
+    motive (node leaf k v (node rl rk rv rr)))
+  (ind : ∀ k v ll lk lv lr rl rk rv rr,
+    motive ll -> motive lr ->
+    motive rl -> motive rr ->
+    motive (node (node ll lk lv lr) k v (node rl rk rv rr)))
+  : ∀ t, motive t :=
+  builder
+where
+  builder (t : STree α) :=
+    match t with
+    | leaf => base
+    | node leaf k v leaf => ind_te k v
+    | node (node ll lk lv lr) k v leaf =>
+      ind_tl k v ll lk lv lr (builder ll) (builder lr)
+    | node leaf k v (node rl rk rv rr) =>
+      ind_tr k v rl rk rv rr (builder rl) (builder rr)
+    | node (node ll lk lv lr) k v (node rl rk rv rr) =>
+      ind k v ll lk lv lr rl rk rv rr (builder ll) (builder lr) (builder rl) (builder rr)
+
+theorem splayBST_equiv (tree : STree α) : BST tree <-> splayBST tree := by
+  constructor
+  . intro h
+    induction tree using STree.inductionOn with
+    | base => constructor
+    | ind_te k v =>
+      apply splayBST.node_e
+    | ind_tl k v ll lk lv lr ihll ihlr =>
+      cases h with -- todo want a tactic to deal with breaking up bst and foralltree
+      | node _ _ _ _ hfl _ hbstl _ =>
+        cases hbstl with
+        | node _ _ _ _ _ _ hbstll hbstlr =>
+          cases hfl with
+          | node _ _ _ _ hfll hineq hflr =>
+            apply splayBST.node_l <;> try simp [*]
+            constructor <;> assumption
+    | ind_tr k v rl rk rv rr ihrl ihrr =>
+      cases h with
+      | node _ _ _ _ _ hfr _ hbstr =>
+        cases hbstr with
+        | node _ _ _ _ _ _ hbstrl hbstrr =>
+          cases hfr with
+          | node _ _ _ _ hfrl hineq hfrr =>
+            apply splayBST.node_r <;> try simp [*]
+            constructor <;> assumption
+    | ind k v ll lk lv lr rl rk rv rr ihll ihlr ihrl ihrr =>
+      cases h with
+      | node _ _ _ _ hfl hfr hbstl hbstr =>
+        cases hfl with
+        | node _ _ _ _ hfll hlk hflr =>
+          cases hfr with
+          | node _ _ _ _ hfrl hrk hfrr =>
+            cases hbstl with
+            | node _ _ _ _ _ _ hbstll hbstlr =>
+              cases hbstr with
+              | node _ _ _ _ _ _ hbstrl hbstrr =>
+                apply splayBST.node_rl <;> (try simp [*]) <;> constructor <;> assumption
+  . intro h
+    induction h with
+    | leaf => constructor
+    | node_e k v =>
+      constructor <;> constructor
+    | node_l k v ll lk lv lr hfll hflr hfl _ _ ihll ihlr =>
+      cases hfl with
+      | node _ _ _ _ hfll2 hlk hflr2 =>
+      constructor <;> constructor <;> assumption
+    | node_r k v rl rk rv rr hfrl hfrr hfr _ _ ihll ihrr =>
+      cases hfr with
+      | node _ _ _ _ hfrl2 hrk hfrr2 =>
+        constructor <;> constructor <;> assumption
+    | node_rl k v ll lk lv lr rl rk rv rr hfll hflr hfrl hfrr hfl hfr _ _ _ _ ihll ihlr ihrl ihrr =>
+      cases hfl with
+      | node _ _ _ _ hfll2 hlk hflr2 =>
+        cases hfr with
+        | node _ _ _ _ hfrl2 hrk hfrr2 =>
+          constructor <;> constructor <;> assumption
+
+theorem splay_bound_equiv (tree : STree α) (key : Nat)
+  : tree.bound key = tree.bound' key := by
+  induction tree using STree.inductionOn with
+  | base => rfl
+  | ind_te k v =>
+    simp
+    by_cases (key = k) <;> simp [*]
+  | ind_tl k v ll lk lv lr ihll ihlr =>
+    simp
+    by_cases' (key = k) h1
+    by_cases' (key < k) h2
+    by_cases' (key = lk) h3
+    by_cases' (key < lk) h4
+    rw [<-ihll]
+    simp
+    match STree.splay ll key with
+    | .leaf => simp; linarith
+    | .node _ _ _ _ => simp
+    rw [<-ihlr]
+    simp
+    match STree.splay lr key with
+    | .leaf => simp; assumption
+    | .node _ _ _ _ => simp
+  | ind_tr k v rl rk rv rr ihrl ihrr =>
+    simp
+    by_cases' (key = k) h1
+    by_cases' (key < k) h2
+    by_cases' (key = rk) h3
+    by_cases' (key < rk) h4
+    rw [<-ihrl]
+    simp
+    match STree.splay rl key with
+    | .leaf => simp; linarith
+    | .node _ _ _ _ => simp
+    rw [<-ihrr]
+    simp
+    match STree.splay rr key with
+    | .leaf => simp; assumption
+    | .node _ _ _ _ => simp
+  | ind k v ll lk lv lr rl rk rv rr ihll ihlr ihrl ihrr =>
+    simp
+    by_cases' (key = k) h1
+    by_cases' (key < k) h2
+    . by_cases' (key = lk) h3
+      by_cases' (key < lk) h4
+      rw [<-ihll]
+      simp
+      match STree.splay ll key with
+      | .leaf => simp; linarith
+      | .node _ _ _ _ => simp
+      rw [<-ihlr]
+      simp
+      match STree.splay lr key with
+      | .leaf => simp; assumption
+      | .node _ _ _ _ => simp
+    . by_cases' (key = rk) h3
+      by_cases' (key < rk) h4
+      rw [<-ihrl]
+      simp
+      match STree.splay rl key with
+      | .leaf => simp; linarith
+      | .node _ _ _ _ => simp
+      rw [<-ihrr]
+      simp
+      match STree.splay rr key with
+      | .leaf => simp; assumption
+      | .node _ _ _ _ => simp    
+
+-- NOTE: revert is a tactic
+
+theorem lookup_equiv (tree : STree α) (key : Nat)
+  : (tree.lookup key).1 = (tree.lookup' key).1 := by
+  induction tree using STree.inductionOn with
+  | base => rfl
+  | ind_te k v => simp; by_cases' (key = k) h
+  | ind_tl k v ll lk lv lr ihll ihlr =>
+    simp at *
+    by_cases' (key = k) h1
+    by_cases' (key < k) h2
+    by_cases' (key = lk) h3
+    by_cases' (key < lk) h4
+    . rw [<-ihll]
+      match ll.splay key with
+      | .leaf => simp [*]
+      | .node _ k' _ _ =>
+        simp
+        by_cases' (key = k') h5
+    . rw [<-ihlr]
+      match lr.splay key with
+      | .leaf => simp [*]
+      | .node _ k' _ _ =>
+        simp
+        by_cases' (key = k') h5
+  | ind_tr k v rl rk rv rr ihrl ihrr =>
+    simp at *
+    by_cases' (key = k) h1
+    by_cases' (key < k) h2
+    by_cases' (key = rk) h3
+    by_cases' (key < rk) h4
+    . rw [<-ihrl]
+      match rl.splay key with
+      | .leaf => simp [*]
+      | .node _ k' _ _ =>
+        simp
+        by_cases' (key = k') h5
+    . rw [<-ihrr]
+      match rr.splay key with
+      | .leaf => simp [*]
+      | .node _ k' _ _ =>
+        simp
+        by_cases' (key = k') h5
+  | ind k v ll lk lv lr rl rk rv rr ihll ihlr ihrl ihrr =>
+    simp at *
+    by_cases' (key = k) h1
+    by_cases' (key < k) h2
+    . by_cases' (key = lk) h3
+      by_cases' (key < lk) h4
+      . rw [<-ihll]
+        match ll.splay key with
+        | .leaf => simp [*]
+        | .node _ k' _ _ =>
+        simp
+        by_cases' (key = k') h5
+      . rw [<-ihlr]
+        match lr.splay key with
+        | .leaf => simp [*]
+        | .node _ k' _ _ =>
+        simp
+        by_cases' (key = k') h5
+    . by_cases' (key = rk) h3
+      by_cases' (key < rk) h4
+      . rw [<-ihrl]
+        match rl.splay key with
+        | .leaf => simp [*]
+        | .node _ k' _ _ =>
+          simp
+          by_cases' (key = k') h5
+      . rw [<-ihrr]
+        match rr.splay key with
+        | .leaf => simp [*]
+        | .node _ k' _ _ =>
+          simp
+          by_cases' (key = k') h5
+
+theorem splay_empty_helper (l r : STree α) (k key : Nat) (v : α) :
+  STree.splay (.node l k v r) key ≠ STree.leaf := by
+  cases l <;> cases r <;> simp [STree.splay] <;> by_cases' (key = k) h <;> by_cases' (key < k) h1
+  . rename_i tl tk tv tr
+    by_cases' (key = tk) h2
+    by_cases' (key < tk) h3
+    case pos =>
+      match STree.splay tl key with
+      | .leaf => simp
+      | .node _ _ _ _ => simp
+    case neg =>
+      match STree.splay tr key with
+      | .leaf => simp
+      | .node _ _ _ _ => simp
+  . rename_i tl tk tv tr
+    by_cases' (key = tk) h2
+    by_cases' (key < tk) h3
+    case pos =>
+      match STree.splay tl key with
+      | .leaf => simp
+      | .node _ _ _ _ => simp
+    case neg =>
+      match STree.splay tr key with
+      | .leaf => simp
+      | .node _ _ _ _ => simp
+  all_goals (rename_i ll lk lv lr rl rk rv rr)
+  . by_cases' (key = lk) h2
+    by_cases' (key < lk) h3
+    match STree.splay ll key with
+    | .leaf => simp
+    | .node _ _ _ _ => simp
+    match STree.splay lr key with
+    | .leaf => simp
+    | .node _ _ _ _ => simp
+  . by_cases' (key = rk) h2
+    by_cases' (key < rk) h3
+    match STree.splay rl key with
+    | .leaf => simp
+    | .node _ _ _ _ => simp
+    match STree.splay rr key with
+    | .leaf => simp
+    | .node _ _ _ _ => simp
+
+theorem splay_empty (t : STree α) (key : Nat) :
+  t = STree.leaf <-> t.splay key = STree.leaf := by
+  constructor
+  . intro h
+    rw [h]
+    rfl
+  . cases t with
+    | leaf => simp
+    | node l k v r =>
+      intro h
+      exfalso
+      apply (splay_empty_helper l r k key v h)
+
+theorem ins_Forall (t : STree α) (key : Nat) (val : α) (p : Nat -> α -> Prop)
+  : ForallTree p t ->
+    p key val ->
+    ForallTree p (t.ins key val) := by
+  induction t with
+  | leaf =>
+    intros
+    simp [STree.ins]
+    constructor <;> assumption
+  | node l k v r ihl ihr =>
+    intro h hp
+    simp [STree.ins]
+    cases h with
+    | node _ _ _ _ hfl hp2 hfr =>
+      by_cases' (key = k) heq
+      . rw [<-heq]
+        constructor <;> assumption
+      . by_cases' (key < k) hlt
+        . constructor <;> simp [*]
+        . constructor <;> simp [*]
+
+theorem ins_BST (t : STree α) (key : Nat) (val : α)
+  : BST t -> BST (t.ins key val) := by
+  intro hbst
+  induction hbst with
+  | leaf => constructor <;> constructor
+  | node l k v r hfl hfr hbstl hbstr ihl ihr =>
+    simp [STree.ins]
+    by_cases' (key = k) heq
+    . constructor <;> simp [*]
+    . by_cases' (key < k) hlt
+      . constructor <;> try assumption
+        apply ins_Forall <;> assumption
+      . constructor <;> try assumption
+        apply ins_Forall <;> try assumption
+        sorry -- linarith can't do this????????
+
+theorem splay_Forall (t : STree α) (key : Nat) (p : Nat -> α -> Prop)
+  : ForallTree p t -> ForallTree p (t.splay key) := by
+  induction t using STree.inductionOn with
+  | base => intro h; simp; assumption
+  | ind_te k v => intro h; simp; assumption
+  | ind_tl k v ll lk lv lr ihll ihlr =>
+    intro h
+    simp
+    by_cases' (key = k) heq
+    by_cases' (key < k) hlt
+    cases h with
+    | node _ _ _ _ hfl hp =>
+      cases hfl with
+      | node _ _ _ _ hfll hpl hflr =>
+        by_cases' (key = lk) heqlk
+        . constructor <;> try assumption
+          constructor <;> assumption
+        . by_cases' (key < lk) hltlk
+          . sorry -- TODO need to destruct but keep equation
+          . sorry -- TODO need to destruct but keep equation
+  | ind_tr k v rl rk rv rr ihrl ihrr =>
+    intro h
+    simp
+    by_cases' (key = k) heq
+    by_cases' (key < k) hlt
+    cases h with
+    | node _ _ _ _ _ hp hfr =>
+      cases hfr with
+      | node _ _ _ _ hfrl hpr hfrr =>
+        by_cases' (key = rk) heqrk
+        . constructor <;> try assumption
+          constructor <;> assumption
+        . by_cases' (key < rk) hltrk
+          . sorry -- TODO need to destruct but keep equation
+          . sorry -- TODO need to destruct but keep equation
+  | ind k v ll lk lv lr rl rk rv rr ihll ihlr ihrl ihrr =>
+    intro h
+    simp
+    by_cases' (key = k) heq
+    cases h with
+    | node _ _ _ _ hfl hp hfr =>
+      by_cases' (key < k) hlt
+      . cases hfl with
+        | node _ _ _ _ hfll hpl hflr =>
+          by_cases' (key = lk) heqlk
+          . constructor <;> try assumption
+            constructor <;> assumption
+          . by_cases' (key < lk) hltlk
+            . sorry -- TODO need to destruct but keep equation
+            . sorry -- TODO need to destruct but keep equation
+      . cases hfr with
+        | node _ _ _ _ hfrl hpr hfrr =>
+          by_cases' (key = rk) heqrk
+          . constructor <;> try assumption
+            constructor <;> assumption
+          . by_cases' (key < rk) hltrk
+            . sorry -- TODO need to destruct but keep equation
+            . sorry -- TODO need to destruct but keep equation
+
+theorem splay_splayBST (t : STree α) (key : Nat)
+  : splayBST t -> splayBST (t.splay key) := by
+  intro h
+  induction h with
+  | leaf => simp; apply splayBST.leaf
+  | node_e k v => simp; apply splayBST.node_e
+  | node_l k v ll lk lv lr hfll hflr hfl hsbstll hsbstlr ihll ihlr =>
+    simp
+    by_cases' (key = k) heq
+    case pos =>
+      apply splayBST.node_l <;> simp [*]
+    case neg =>
+      by_cases' (key < k) hlt
+      case pos =>
+        cases hfl with
+        | node _ _ _ _ hfll2 hlk hflr2 => 
+          by_cases' (key = lk) hlkeq
+          . rw [<-splayBST_equiv]
+            constructor
+            . assumption
+            . constructor <;> try assumption
+              constructor
+            . rw [splayBST_equiv]; assumption
+            . constructor
+              assumption
+              constructor
+              rw [splayBST_equiv]; assumption
+              constructor
+          . by_cases' (key < lk) hlklt
+            . match ll.splay key with
+              | .leaf =>
+                simp
+                rw [<-splayBST_equiv]
+                constructor
+                assumption
+                constructor
+                assumption
+                assumption
+                constructor
+                rw [splayBST_equiv]; assumption
+                constructor
+                assumption
+                constructor
+                rw [splayBST_equiv]; assumption
+                constructor
+              | .node lll llk llv llr =>
+                simp
+                rw [<-splayBST_equiv]
+                constructor
+                -- TODO lost info here: ll.splay key = .node lll llk llv llr
+                sorry
+                sorry
+                sorry
+                constructor
+                sorry
+                constructor
+                assumption
+                assumption
+                constructor
+                sorry
+                constructor
+                assumption
+                constructor
+                rw [splayBST_equiv]; assumption
+                constructor
+            . sorry -- gonna lose information unless I can destruct and keep the equality
+      case neg =>
+        apply splayBST.node_l <;> assumption
+  | node_r k v rl rk rv rr hfrl hfrr hfr hsbstrl hsbstrr ihrl ihrr => sorry
+  | node_rl k v ll lk lv lr rl rk rv rr hfll hflr hfrl hfrr hfl hfr hsbstll hsbstlr hbstrl hbstrr ihll ihlr ihrl ihrr => sorry
+
+theorem splay_BST (t : STree α) (key : Nat)
+  : BST t -> BST (t.splay key) := by
+  intro h
+  rw [splayBST_equiv] at *
+  apply splay_splayBST
+  assumption
+
+theorem insert_BST (t : STree α) (key : Nat) (val : α)
+  : BST t -> BST (t.insert key val) := by
+  intro h
+  unfold STree.insert
+  apply splay_BST
+  apply ins_BST
+  assumption
+
+------- TODO section doc; model verification -------
+
+------- TODO section doc; algebraic spec -------
 
